src/Cvm_Impl.v
@@ -10,10 +10,7 @@ Require Import List.
 Import ListNotations.
 
 (** Monadic CVM implementation *)
-(* TODO: rename this to something besides "copland_compile".  Is really 
-   more of an interpreter.  The Term to Core_Term translation function 
-   is closer to a Copland Compiler than this.  *)
-Fixpoint copland_compile (t:Core_Term): CVM unit :=
+Fixpoint build_cvm (t:Core_Term): CVM unit :=
   match t with
   | aspc a =>
       e <- do_prim a ;;
@@ -23,22 +20,22 @@ Fixpoint copland_compile (t:Core_Term): CVM unit :=
     e' <- doRemote t' q e ;;
     put_ev e'
   | lseqc t1 t2 =>
-      copland_compile t1 ;;
-      copland_compile t2
+      build_cvm t1 ;;
+      build_cvm t2
   | bseqc t1 t2 =>
     split_ev ;;
     e <- get_ev ;;
-    copland_compile t1 ;;
+    build_cvm t1 ;;
     e1r <- get_ev ;;
     put_ev e ;;
-    copland_compile t2 ;;
+    build_cvm t2 ;;
     e2r <- get_ev ;;
     join_seq e1r e2r
   | bparc loc t1 t2 =>
     split_ev ;;
     e <- get_ev ;;
     start_par_thread loc t2 e ;;
-    copland_compile t1 ;;
+    build_cvm t1 ;;
     e1r <- get_ev ;;
     e2r <- wait_par_thread loc t2 e ;;
     join_seq e1r e2r
