src/Cvm_Run.v
@@ -3,7 +3,7 @@
 Require Import Term_Defs Anno_Term_Defs Cvm_Impl Cvm_St StMonad_Coq.
 
 Definition run_cvm (t:Core_Term) st : cvm_st :=
-  execSt (copland_compile t) st.
+  execSt (build_cvm t) st.
 
 Definition run_cvm' (t:Term) st : cvm_st :=
-  run_cvm (term_to_core_term t) st.
+  run_cvm (copland_compile t) st.
