src/IO_Stubs.v
@@ -1,30 +1,37 @@
-(** Abstract definitions of IO Stub signatures.  The functions with names that 
-    have a tick at the end (i.e. do_asp') should be instantiated to concrete 
-    IO functions in the executable language upon extraction.
+(** Abstract definitions of IO Stub signatures.  The functions with monadic 
+    return types (i.e. do_asp') can be replaced by concrete monadic functions
+    in the target language upon extraction.  Alternatively,
+    if the target language does not have built-in monadic support, one can
+    instantiate the non-monadic versions of the stubs instead (i.e. do_asp).
 
-    The non-ticked functions (i.e. do_asp) only live in Coq, and largely 
-    represent raw evidence values.  We leave these  abstract (Admitted) in Coq 
+    The non-monadic stubs (i.e. do_asp) remain abstract (Admitted) in Coq 
     because they are either too low-level to reason about, or require external 
-    IO capabilities not modeled first-class in our spec.  These abstract 
-    evidence values support specification of correctness properties for 
-    Appraisal (see usage of do_asp in appEvent_EvidenceC of Appraisal_Defs.v).
+    IO capabilities not modeled first-class in our spec.  The abstract binary
+    and evidence value results support specification of correctness properties 
+    for Appraisal (see usage of do_asp in appEvent_EvidenceC of 
+    Appraisal_Defs.v).        
  *)
 
 Require Import Term_Defs ConcreteEvidence StMonad_Coq IO_Type.
 
+(** * Stub to encode a sequence of BS values to a single BS value.
+      Real implmenetation will depend on the instantition of BS *)
 Definition encodeEvRaw(e:RawEv): BS.
 Admitted.
 
+(** * Stub for invoking external ASP procedures.  
+      Extracted code should not need to use the Plc or Event_ID parameters 
+      (those can be erased upon extraction). *)
 Definition do_asp (params :ASP_PARAMS) (e:RawEv) (mpl:Plc) (x:Event_ID) : BS.
 Admitted.
 
+(** * Stub for completing a remote communication session with an external AM. *)
 Definition doRemote_session (t:Term) (pTo:Plc) (e:EvC) : EvC.
 Admitted.
 
-
-
-
-
+(** * Stub to simulate evidence collected by a parallel CVM instance *)
+Definition parallel_vm_thread (l:Loc) (t:Core_Term) (p:Plc) (e:EvC) : EvC.
+Admitted.
 
 
 Definition do_asp' (params :ASP_PARAMS) (e:RawEv) (mpl:Plc) (x:Event_ID) : IO BS :=
@@ -36,25 +43,5 @@ Definition doRemote_session' (t:Term) (pTo:Plc) (e:EvC) : IO EvC :=
 Definition do_start_par_thread (loc:Loc) (t:Core_Term) (e:RawEv) : IO unit :=
   ret tt.
 
-Definition parallel_vm_thread (l:Loc) (t:Core_Term) (p:Plc) (e:EvC) : EvC.
-Admitted.
-
 Definition do_wait_par_thread (loc:Loc) (t:Core_Term) (p:Plc) (e:EvC) : IO EvC :=
   ret (parallel_vm_thread loc t p e).
-
-
-
-
-(*
-Definition do_sig (bs:BS) (p:Plc) (sigTag:Event_ID) : BS.
-Admitted.
-
-Definition do_sig' (bs:BS) (p:Plc) (sigTag:Event_ID) : IO BS :=
-  ret (do_sig bs p sigTag).
-
-Definition do_hash (bs:BS) (p:Plc) : BS.
-Admitted.
-
-Definition do_hash' (bs:BS) (p:Plc) : IO BS :=
-  ret (do_hash bs p).
-*)
